\documentclass{beamer}

\usepackage[english]{babel}
\usepackage{graphicx}% or whatever
\usepackage{amsmath}
\usepackage{amssymb}
\usepackage[utf8]{inputenc}
% or whatever

\usepackage{times}
\usepackage[T1]{fontenc}
% Or whatever. Note that the encoding and the font should match. If T1

\begin{document}
%----------------------------------------------------------------------------------------------%
\begin{frame}
\frametitle{Recurrence Relations : Proof by Induction}
\Large
\vspace{-1cm}
\begin{itemize}
\item A sequence is determined by the recurrence relation $u_{n+1} = 3u_n+2$ and initial term $u_1 =2$.
\item Prove by induction the following statement, for all $n \in \mathbb{Z^{+}}$.
\[ u_n=3^n-1\]
\end{itemize}
\end{frame}
%----------------------------------------------------------------------------------------------%
\begin{frame}
\frametitle{Recurrence Relations : Proof by Induction}
\Large
\vspace{-1cm}
\textbf{Step 1 : Base Step}
\begin{itemize}
\item Demonstrate the expression is valid for $n=1$ ( i.e. $u_1$ = 2).
\[ u_n=3^n-1  \]
\[ u_1=3^1-1 \]
\[ u_1=3 -1 = 2 \]
\end{itemize}
\end{frame}
%----------------------------------------------------------------------------------------------%
\begin{frame}
\frametitle{Recurrence Relations : Proof by Induction}
\Large
\vspace{-1cm}
\textbf{Step 2 : Induction Hypothesis}
\begin{itemize}
\item Demonstrate the expression is valid for $n=k$ .
\[ u_k=3^k-1 \]

\end{itemize}
\end{frame}
%----------------------------------------------------------------------------------------------%
\begin{frame}
\frametitle{Recurrence Relations : Proof by Induction}
\Large
\vspace{-1cm}
\textbf{Step 3 : Induction Step}
\begin{itemize}
\item Demonstrate the expression is valid for $n=k+1$ .
\[ u_{k+1}=3^{k+1}-1 \]
\[ u_{k+1}=3.3^{k}-1 \]
\[ u_{k+1}=(1+2).3^{k}-1 \]
\[ u_{k+1}=3^{k} + 2.3^{k}-1 \]
\end{itemize}
\end{frame}
%----------------------------------------------------------------------------------------------%
\end{document}
